Test/git-issues/git-issue-032-errors.dfy
@@ -5,12 +5,12 @@
 method errors() {
   var e := ();
   var x := (2,3);
-  match x { case () => print "OK"; case _ => print "BAD"; }
-  match e { case (a,b) => print "OK"; case _ => print "BAD"; }
-  match () { case (a,b) => print "OK"; case _ => print "BAD"; }
-  var z := match x { case () => 0 case _ => 1};
-  var y := match e { case (a,b) => 0 case _ => 1};
-  var w := match () { case (a,b) => 0 case _ => 1};
+  match x { case () => print "OK"; case _ => print "BAD"; }  // ERROR
+  match e { case (a,b) => print "OK"; case _ => print "BAD"; } // ERROR
+  match () { case (a,b) => print "OK"; case _ => print "BAD"; } // ERROR
+  var z := match x { case () => 0 case _ => 1}; // ERROR
+  var y := match e { case (a,b) => 0 case _ => 1}; // ERROR
+  var w := match () { case (a,b) => 0 case _ => 1}; // ERROR
 }
 
 
